Added a couple of additional lens laws and switched blocks to use symmetric lenses

utp/examples/local_var.thy
@@ -4,23 +4,35 @@ theory local_var
   imports "UTP.utp"
 begin
 
+text \<open> State space of global variables. \<close>
+
 alphabet global =
   x :: int
   y :: int
 
+text \<open> State space of local variables, extending @{typ global} with an additional variable. \<close>
+
 alphabet local = global +
   temp :: int
 
+text \<open> Construct a symmetric lens that partitions the state space into globals and locals, using
+  the lenses @{term global.base\<^sub>L} and @{term global.more\<^sub>L}. \<close>
+
+abbreviation "lv \<equiv> \<lparr> view = (global.base\<^sub>L :: (global \<Longrightarrow> local)), coview = global.more\<^sub>L \<rparr>"
+
+lemma sym_lens_lv [simp]: "sym_lens lv"
+  by (rule sym_lens.intro, simp_all)
+
+text \<open> Define a program that uses the symmetric lens for modelling the variable scope \<close>
+
 abbreviation swap :: "global hrel" where
-"swap \<equiv> open\<^bsub>global.base\<^sub>L :: global \<Longrightarrow> local\<^esub> ;; \<comment> \<open> Open the local scope \<close>
+"swap \<equiv> open\<^bsub>lv\<^esub> ;; \<comment> \<open> Open the local scope \<close>
          temp := &x ;; \<comment> \<open> @{term x} is a global variable; @{term temp} is a local variable\<close> 
          x := &y ;; 
          y := &temp ;; 
-         close\<^bsub>global.base\<^sub>L\<^esub>" \<comment> \<open> Close the local scope\<close>
+         close\<^bsub>lv\<^esub>" \<comment> \<open> Close the local scope\<close>
 
-lemma "\<lbrace>&x =\<^sub>u \<guillemotleft>X\<guillemotright> \<and> &y =\<^sub>u \<guillemotleft>Y\<guillemotright>\<rbrace>
-        open\<^bsub>global.base\<^sub>L\<^esub> ;; temp := &x ;; x := &y ;; y := &temp ;; close\<^bsub>global.base\<^sub>L\<^esub>
-       \<lbrace>&x =\<^sub>u \<guillemotleft>Y\<guillemotright> \<and> &y =\<^sub>u \<guillemotleft>X\<guillemotright>\<rbrace>\<^sub>u"
+lemma "\<lbrace>&x =\<^sub>u \<guillemotleft>X\<guillemotright> \<and> &y =\<^sub>u \<guillemotleft>Y\<guillemotright>\<rbrace> swap \<lbrace>&x =\<^sub>u \<guillemotleft>Y\<guillemotright> \<and> &y =\<^sub>u \<guillemotleft>X\<guillemotright>\<rbrace>\<^sub>u"
   unfolding block_open_def block_close_def
   by (rel_auto)
 
