utp/utp_blocks.thy
@@ -1,64 +1,74 @@
-section \<open> Blocks \<close>
+section \<open> Blocks (Abstract Local Variables) \<close>
 
 theory utp_blocks
   imports utp_rel_laws
 begin
 
+syntax
+  "_slens_view" :: "logic \<Rightarrow> svid" ("\<V>[_]")
+
+translations
+  "_slens_view a" => "\<V>\<^bsub>a\<^esub>"
+
 subsection \<open> Extending and Contracting Substitutions \<close>
 
-definition subst_ext :: "('\<alpha> \<Longrightarrow> '\<beta>) \<Rightarrow> ('\<alpha>, '\<beta>) psubst" ("ext\<^sub>s") where
-[upred_defs]: "ext\<^sub>s a = \<lparr>\<^bold>v \<mapsto>\<^sub>s &\<^bold>v \<restriction>\<^sub>e a\<rparr>"
+definition subst_ext :: "(<'\<alpha>, '\<beta>> \<Longleftrightarrow> '\<gamma>) \<Rightarrow> ('\<alpha>, '\<gamma>) psubst" ("ext\<^sub>s") where
+"ext\<^sub>s a = (\<lambda> s. create\<^bsub>\<V>\<^bsub>a\<^esub>\<^esub> s)" \<comment> \<open> Extend state space by execution of create \<close>
 
-definition subst_con :: "('\<alpha> \<Longrightarrow> '\<beta>) \<Rightarrow> ('\<beta>, '\<alpha>) psubst" ("con\<^sub>s") where
-[upred_defs]: "con\<^sub>s a = \<lparr>\<^bold>v \<mapsto>\<^sub>s &\<^bold>v \<oplus>\<^sub>p a\<rparr>"
+lemma subst_ext_alt_def [upred_defs]: "ext\<^sub>s a = \<lparr>\<^bold>v \<mapsto>\<^sub>s &\<^bold>v \<restriction>\<^sub>e \<V>\<^bsub>a\<^esub>\<rparr>"
+  unfolding subst_ext_def by (rel_auto)
 
-lemma subst_res_ext_con: "\<sigma> \<restriction>\<^sub>s a = con\<^sub>s a \<circ> \<sigma> \<circ> ext\<^sub>s a"
+definition subst_con :: "(<'\<alpha>, '\<beta>> \<Longleftrightarrow> '\<gamma>) \<Rightarrow> ('\<gamma>, '\<alpha>) psubst" ("con\<^sub>s") where
+"con\<^sub>s a = (\<lambda> s. get\<^bsub>\<V>\<^bsub>a\<^esub>\<^esub> s)" \<comment> \<open> Contract the state space with get \<close>
+
+lemma subst_con_alt_def [upred_defs]: "con\<^sub>s a = \<lparr>\<^bold>v \<mapsto>\<^sub>s &\<^bold>v \<oplus>\<^sub>p \<V>\<^bsub>a\<^esub>\<rparr>"
+  unfolding subst_con_def by (rel_auto)
+
+lemma subst_res_ext_con: "\<sigma> \<restriction>\<^sub>s (\<V>\<^bsub>a\<^esub>) = con\<^sub>s a \<circ> \<sigma> \<circ> ext\<^sub>s a"
   by (rel_simp)
 
-lemma subst_ext_con [usubst]: "mwb_lens a \<Longrightarrow> con\<^sub>s a \<circ> ext\<^sub>s a = id"
+lemma subst_ext_con [usubst]: "psym_lens a \<Longrightarrow> con\<^sub>s a \<circ> ext\<^sub>s a = id"
   by (rel_simp)
+
+text \<open> Variables in the "global" state space will be retained after a state is contracted \<close>
 
 lemma subst_con_update_sublens [usubst]: 
-  "\<lbrakk> mwb_lens a; x \<subseteq>\<^sub>L a \<rbrakk> \<Longrightarrow> con\<^sub>s a \<circ> subst_upd \<sigma> x v = subst_upd (con\<^sub>s a \<circ> \<sigma>) (x /\<^sub>L a) v"
+  "\<lbrakk> psym_lens a; x \<subseteq>\<^sub>L \<V>\<^bsub>a\<^esub> \<rbrakk> \<Longrightarrow> con\<^sub>s a \<circ> subst_upd \<sigma> x v = subst_upd (con\<^sub>s a \<circ> \<sigma>) (x /\<^sub>L \<V>\<^bsub>a\<^esub>) v"
   by (simp add: subst_con_def usubst alpha, rel_simp)
 
-lemma subst_con_update_indep [usubst]: 
-  "\<lbrakk> mwb_lens x; mwb_lens a; a \<bowtie> x \<rbrakk> \<Longrightarrow> con\<^sub>s a \<circ> subst_upd \<sigma> x v = (con\<^sub>s a \<circ> \<sigma>)"
-  by (simp add: subst_con_def usubst alpha)
+text \<open> Variables in the "local" state space will be lost after a state is contracted \<close>
 
-lemma subst_ext_apply [usubst]: "\<langle>ext\<^sub>s a\<rangle>\<^sub>s x = &x \<restriction>\<^sub>e a"
+lemma subst_con_update_indep [usubst]: 
+  "\<lbrakk> mwb_lens x; psym_lens a; \<V>\<^bsub>a\<^esub> \<bowtie> x \<rbrakk> \<Longrightarrow> con\<^sub>s a \<circ> subst_upd \<sigma> x v = (con\<^sub>s a \<circ> \<sigma>)"
+  by (simp add: subst_con_alt_def usubst alpha)
+
+lemma subst_ext_apply [usubst]: "\<langle>ext\<^sub>s a\<rangle>\<^sub>s x = &x \<restriction>\<^sub>e \<V>\<^bsub>a\<^esub>"
   by (rel_simp)
 
 subsection \<open> Generic Blocks \<close>
 
-definition block_open :: "('a \<Longrightarrow> 'b) \<Rightarrow> ('a, 'b) urel" ("open\<^bsub>_\<^esub>") where
-[upred_defs]: "block_open a = \<langle>ext\<^sub>s a\<rangle>\<^sub>a ;; ($a\<acute> =\<^sub>u $a)"
+text \<open> We ensure that the initial values of local are arbitrarily chosen \<close>
 
-definition block_close :: "('a \<Longrightarrow> 'b) \<Rightarrow> ('b, 'a) urel" ("close\<^bsub>_\<^esub>") where
+definition block_open :: "(<'a, 'c> \<Longleftrightarrow> 'b) \<Rightarrow> ('a, 'b) urel" ("open\<^bsub>_\<^esub>") where
+[upred_defs]: "block_open a = \<langle>ext\<^sub>s a\<rangle>\<^sub>a ;; ($\<V>[a]\<acute> =\<^sub>u $\<V>[a])"
+
+definition block_close :: "(<'a, 'c> \<Longleftrightarrow> 'b) \<Rightarrow> ('b, 'a) urel" ("close\<^bsub>_\<^esub>") where
 [upred_defs]: "block_close a = \<langle>con\<^sub>s a\<rangle>\<^sub>a"
 
 lemma block_open_conv: 
-  "mwb_lens a \<Longrightarrow> open\<^bsub>a\<^esub>\<^sup>- = close\<^bsub>a\<^esub>"
+  "psym_lens a \<Longrightarrow> open\<^bsub>a\<^esub>\<^sup>- = close\<^bsub>a\<^esub>"
   by (rel_auto)
 
 lemma block_open_close:
-  "mwb_lens a \<Longrightarrow> open\<^bsub>a\<^esub> ;; close\<^bsub>a\<^esub> = II"
-  by (rel_auto, metis mwb_lens_def weak_lens.create_get)
-
-lemma block_open_open:
-  "\<lbrakk> mwb_lens a; mwb_lens b\<rbrakk> \<Longrightarrow> open\<^bsub>a\<^esub> ;; open\<^bsub>b\<^esub> = open\<^bsub>a ;\<^sub>L b\<^esub>"
-  by (rel_auto)
-
-lemma block_close_close:
-  "\<lbrakk> mwb_lens a; mwb_lens b\<rbrakk> \<Longrightarrow> close\<^bsub>a\<^esub> ;; close\<^bsub>b\<^esub> = close\<^bsub>b ;\<^sub>L a\<^esub>"
-  by (rel_auto)
+  "psym_lens a \<Longrightarrow> open\<^bsub>a\<^esub> ;; close\<^bsub>a\<^esub> = II"
+  by (rel_auto, metis mwb_lens_def psym_lens.mwb_region weak_lens.create_get)
 
 lemma block_assigns_open:
-  "vwb_lens a \<Longrightarrow> \<langle>\<sigma>\<rangle>\<^sub>a ;; open\<^bsub>a\<^esub> = open\<^bsub>a\<^esub> ;; \<langle>\<sigma> \<oplus>\<^sub>s a\<rangle>\<^sub>a"
-  by (rel_auto, metis lens_override_def lens_override_idem mwb_lens_axioms_def mwb_lens_def vwb_lens_def weak_lens.put_get)
+  "sym_lens a \<Longrightarrow> \<langle>\<sigma>\<rangle>\<^sub>a ;; open\<^bsub>a\<^esub> = open\<^bsub>a\<^esub> ;; \<langle>\<sigma> \<oplus>\<^sub>s \<V>\<^bsub>a\<^esub>\<rangle>\<^sub>a"
+  by (rel_auto, metis mwb_lens_axioms_def mwb_lens_def sym_lens_def vwb_lens_def wb_lens_axioms_def wb_lens_def weak_lens.put_get)
 
 lemma block_assign_local_close:
-  "a \<bowtie> x \<Longrightarrow> x := v ;; close\<^bsub>a\<^esub> = close\<^bsub>a\<^esub>"
+  "\<V>\<^bsub>a\<^esub> \<bowtie> x \<Longrightarrow> x := v ;; close\<^bsub>a\<^esub> = close\<^bsub>a\<^esub>"
   by (rel_auto)
 
 end
